Prove that Stenning program refines the model

fairneris/examples/stenning_code.v
@@ -15,13 +15,13 @@ Definition client (sa_clt sa_srv : socket_address) : val :=
      SocketBind "sh_clt" #sa_clt;;
      SetReceiveTimeout "sh_clt" #1 #1;;
      let: "go" := (rec: "f" "i" :=
-        SendTo "sh_clt" "sa_srv" (i2s "i");;
+        SendTo "sh_clt" (i2s "i") #sa_srv ;;
         match: (ReceiveFrom "sh_clt") with
           NONE     => "f" "i"
-        | SOME "m" => if: Snd "m" = "sa_srv"
+        | SOME "m" => if: Snd "m" = #sa_srv
                       then
                         let: "j" := s2i (Fst "m") in
-                        if: "i" = "j"
+                        if: InjR "i" = "j"
                         then "f" ("i" + #1)
                         else "f" "i"
                       else
@@ -37,12 +37,12 @@ Definition server (sa_clt sa_srv : socket_address) : val :=
      let: "go" := (rec: "f" "j" :=
         match: (ReceiveFrom "sh_srv") with
           NONE     => "f" "j"
-        | SOME "m" => if: Snd "m" = "sa_clt"
+        | SOME "m" => if: Snd "m" = #sa_clt
                       then
                         let: "i" := s2i (Fst "m") in
-                        if: "j"+#1 = "i"
-                        then SendTo "sh_srv" "sa_clt" "i";; "f" "i"
-                        else SendTo "sh_srv" "sa_clt" "j";; "f" "j"
+                        if: InjR ("j"+#1) = "i"
+                        then SendTo "sh_srv" (i2s (#1 + "j")) #sa_clt ;; "f" (#1 + "j")
+                        else SendTo "sh_srv" (i2s "j") #sa_clt ;; "f" "j"
                       else
                         "f" "j"
         end)
@@ -97,13 +97,13 @@ Section with_Σ.
 
   Lemma wp_client tid (f : nat) (Hf: f > 40) :
     {{{ inv Ns retinv ∗ is_node ipA ∗ saA ⤇ (λ msg, ⌜ msg = msg⌝) ∗ saB ⤇ (λ msg, ⌜ msg = msg⌝) ∗
-          own stenning_A_name (◯E (AReceiving 0)) ∗
+          own stenning_A_name (◯E (ASending 0)) ∗
           (ipA, tid) ↦M {[ Arole := f ]} ∗ saA ⤳ (∅, ∅) ∗
           free_ports (ip_of_address saA) {[port_of_address saA]} }}}
       (mkExpr (ip_of_address saA) (client saA saB #())) @ (ipA, tid); ⊤
     {{{ v, RET v; (ipA, tid) ↦M ∅ }}}.
   Proof.
-    iIntros (Φ) "(Hinv&#Hin&HsA&HsB&Hst&Hf&HRT&Hfp) HΦ".
+    iIntros (Φ) "(#Hinv&#Hin&#HsA&#HsB&Hst&Hf&HRT&Hfp) HΦ".
     rewrite /client.
     wp_pure _.
 
@@ -136,18 +136,272 @@ Section with_Σ.
     iAssert (∃ R T, saA ⤳ (R, T))%I with "[HRT]" as (R T) "HRT".
     { iExists _, _. iFrame. }
 
-    (* TODO: generalize 0 *)
-    iLöb as "IH" forall (f' R T) "Hf".
-  Admitted.
+    remember 0 as n eqn:Heq.
+    replace (ASending 0) with (ASending n); last naive_solver.
+
+    assert (n >= 0) as Hn; first lia. clear Heq.
+    iLöb as "IH" forall (f' n Hn R T) "Hf". iDestruct "Hf'" as %Hf.
+
+    wp_pure _.
+    wp_pure _.
+
+    wp_bind (SendTo _ _ _).
+    iApply sswp_MU_wp_fupd.
+
+    iInv Ns as "Hi" "Hclose". iModIntro.
+    iApply (wp_send _ _ false with "[Hsh] [HRT] [HsA]")=>//=>//=>//.
+    iNext. iIntros "Hsh HRT".
+    iDestruct "Hi" as "(Hfr & %stA & %stB & Hmod & HstA & HstB)".
+    iDestruct (token_agree with "HstA Hst") as %->.
+
+    iApply (mu_step_model _ _ _ _ ∅ ∅ _ ((AReceiving n, stB) : stenning_model) with "Hmod [Hf] [Hfr //]").
+    { simpl. constructor. }
+    { set_solver. }
+    { set_solver. }
+    { rewrite fmap_empty map_union_empty. done. }
+    iIntros "Hmod Hf Hfr".
+
+    iMod (token_update with "[$HstA $Hst]") as "[HstA Hst]".
+    iMod ("Hclose" with "[Hfr Hmod HstA HstB]").
+    { iNext. rewrite /retinv. iFrame. iExists (AReceiving n), _. iFrame. }
+    rewrite map_union_empty /usr_fl /=. iModIntro. iApply wp_value'. do 2 wp_pure _.
+
+    wp_bind (ReceiveFrom _).
+    iApply sswp_MU_wp_fupd.
+    iInv Ns as "Hi" "Hclose". iModIntro.
+
+    iApply (wp_recv with "[Hsh] [HRT] [HsB]")=>//=>//=>//.
+    iNext. clear stB. iDestruct "Hi" as "(Hfr & %stA & %stB & Hmod & HstA & HstB)".
+    iDestruct (token_agree with "HstA Hst") as %->.
+
+    iIntros (om r) "Hmsg".
+
+    iAssert (⌜ ∃ omsg, om = Recv saA omsg ⌝)%I as %[omsg ->].
+    { iDestruct "Hmsg" as "[(-> & -> & Hsh & HRT)|(%msg & -> & -> & %Heqdest & Hsh & HRT & Hnew)]";
+      iPureIntro; naive_solver. }
+    destruct (decide (good_message false n omsg)) as [[msg Hgood]|Hbad].
+    - iDestruct "Hmsg" as "[(-> & %Heq & Hsh & HRT)|(%msg' & -> & %Heq & %Heqdest & Hsh & HRT & Hnew)]".
+      { simplify_eq. naive_solver. }
+      destruct Hgood as (?&Hbody&?&?). simplify_eq.
+      iApply (mu_step_model _ _ _ _ ∅ ∅ _ ((ASending (1+n), stB) : stenning_model) with "Hmod [Hf] [Hfr //]").
+      { constructor. exists msg'. naive_solver. }
+      { set_solver. }
+      { set_solver. }
+      { rewrite fmap_empty map_union_empty. done. }
+      iIntros "Hmod Hf Hfr".
+      rewrite map_union_empty /usr_fl /=.
+      iMod (token_update with "[$HstA $Hst]") as "[HstA Hst]".
+      iMod ("Hclose" with "[Hfr Hmod HstA HstB]").
+      { iNext. rewrite /retinv. iFrame. iExists (ASending (1+n)), _. iFrame. }
+      iModIntro. iApply wp_value'. do 5 wp_pure _.
+      rewrite bool_decide_true; last by do 2 f_equal.
+      do 3 wp_pure _.
+      { simpl. rewrite Hbody //. }
+      do 4 wp_pure _. rewrite bool_decide_true //. do 2 wp_pure _.
+      iApply ("IH" with "[] [Hst] [$] [$] [] [$HRT] [$]").
+      { iPureIntro; lia. }
+      { rewrite Z.add_comm //. }
+      { iPureIntro; lia. }
+    - iApply (mu_step_model _ _ _ _ ∅ ∅ _ ((ASending n, stB) : stenning_model) with "Hmod [Hf] [Hfr //]").
+      { simpl. by apply A_RecvFail. }
+      { set_solver. }
+      { set_solver. }
+      { rewrite fmap_empty map_union_empty. done. }
+      iIntros "Hmod Hf Hfr".
+      rewrite map_union_empty /usr_fl /=.
+      iMod (token_update with "[$HstA $Hst]") as "[HstA Hst]".
+      iMod ("Hclose" with "[Hfr Hmod HstA HstB]").
+      { iNext. rewrite /retinv. iFrame. iExists (ASending n), _. iFrame. }
+      iModIntro. iApply wp_value'. simpl.
+      iDestruct "Hmsg" as "[(-> & %Heq & Hsh & HRT)|(%msg & -> & %Heq & %Heqdest & Hsh & HRT & Hnew)]".
+      + do 3 wp_pure _. iApply ("IH" with "[] [Hst] [$] [$] [] [$HRT] [$]")=>//.
+      + do 5 wp_pure _. destruct (decide (m_sender msg = saB)); last first.
+        { rewrite bool_decide_false; last naive_solver. wp_pure _.
+          iApply ("IH" with "[] [Hst] [$] [$] [] [$HRT] [$]")=>//. }
+        rewrite bool_decide_true //; last by do 2 f_equal. do 2 wp_pure _.
+        destruct (ZOfString (m_body msg)) as [msg_n|] eqn:Heqmsg; last first.
+        { wp_pure _. rewrite /= Heqmsg //. do 5 wp_pure _.
+          iApply ("IH" with "[] [Hst] [$] [$] [] [$HRT] [$]")=>//. }
+        wp_pure _. rewrite /= Heqmsg //. do 4 wp_pure _.
+        rewrite bool_decide_false; last first.
+        { intros Hc. simplify_eq. apply Hbad. eexists; split=>//. }
+        wp_pure _. iApply ("IH" with "[] [Hst] [$] [$] [] [$HRT] [$]")=>//.
+  Qed.
 
   Lemma wp_sever tid (f : nat) (Hf: f > 40) :
-    {{{ inv Ns retinv ∗ is_node ipA ∗ saA ⤇ (λ msg, ⌜ msg = msg⌝) ∗ saB ⤇ (λ msg, ⌜ msg = msg⌝) ∗
+    {{{ inv Ns retinv ∗ is_node ipB ∗ saA ⤇ (λ msg, ⌜ msg = msg⌝) ∗ saB ⤇ (λ msg, ⌜ msg = msg⌝) ∗
           own stenning_B_name (◯E (BReceiving 0)) ∗
           (ipB, tid) ↦M {[ Brole := f ]} ∗ saB ⤳ (∅, ∅) ∗
-          free_ports (ip_of_address saA) {[port_of_address saA]} }}}
-      (mkExpr (ip_of_address saA) (server saA saB)) @ (ipA, tid); ⊤
-    {{{ v, RET v; (ipA, tid) ↦M ∅ }}}.
+          free_ports (ip_of_address saB) {[port_of_address saB]} }}}
+      (mkExpr (ip_of_address saB) (server saA saB #())) @ (ipB, tid); ⊤
+    {{{ v, RET v; (ipB, tid) ↦M ∅ }}}.
   Proof.
-  Admitted.
+    iIntros (Φ) "(#Hinv&#Hin&#HsA&#HsB&Hst&Hf&HRT&Hfp) HΦ".
+    rewrite /server.
+    wp_pure _.
 
+    wp_bind (NewSocket _).
+    iApply sswp_MU_wp. iApply wp_new_socket=>//.
+    iIntros (sh) "Hsh".
+    mu_fuel.
+
+    iApply wp_value'. do 2 wp_pure _.
+
+    wp_bind (SocketBind _ _).
+    iApply sswp_MU_wp. iApply (wp_socketbind with "[Hfp] [Hsh]") =>//=; first done.
+    iIntros "Hsh".
+    mu_fuel.
+    iApply wp_value'.
+    do 2 wp_pure _.
+
+    wp_bind (SetReceiveTimeout _ _ _).
+    iApply sswp_MU_wp. iApply (wp_rcvtimeo_ublock NotStuck ⊤ (ipB, tid) sh _ saB 1 1 with "[Hsh]").
+    3: { auto. }
+    { done. }
+    { lia. }
+    iIntros "Hsh". mu_fuel. iApply wp_value'. do 5 wp_pure _.
+
+    iAssert (∃ (f : nat), ⌜ f > 25 ⌝ ∗ (ipB, tid) ↦M <[Brole:=f]> ∅)%I
+      with "[Hf]" as (f') "[Hf' Hf]".
+    { iExists _. iFrame. iPureIntro. lia. }
+    clear f Hf.
+
+    iAssert (∃ R T, saB ⤳ (R, T))%I with "[HRT]" as (R T) "HRT".
+    { iExists _, _. iFrame. }
+
+    remember (-1) as n eqn:Heq.
+    replace (BReceiving 0) with (BReceiving (1+n)); last naive_solver.
+
+    assert (n >= -1) as Hn; first lia. clear Heq.
+    iLöb as "IH" forall (f' n Hn R T) "Hf". iDestruct "Hf'" as %Hf.
+
+    wp_pure _.
+
+    wp_bind (ReceiveFrom _).
+    iApply sswp_MU_wp_fupd.
+    iInv Ns as "Hi" "Hclose". iModIntro.
+
+    iApply (wp_recv with "[Hsh] [HRT] [HsA]")=>//=>//=>//.
+    iNext. iDestruct "Hi" as "(Hfr & %stA & %stB & Hmod & HstA & HstB)".
+    iDestruct (token_agree with "HstB Hst") as %->.
+
+    iIntros (om r) "Hmsg".
+
+    iAssert (⌜ ∃ omsg, om = Recv saB omsg ⌝)%I as %[omsg ->].
+    { iDestruct "Hmsg" as "[(-> & -> & Hsh & HRT)|(%msg & -> & -> & %Heqdest & Hsh & HRT & Hnew)]";
+      iPureIntro; naive_solver. }
+    destruct (decide (good_message true (1+n) omsg)) as [[msg Hgood]|Hbad];
+    [|destruct (decide (omsg = None ∨ (∃ msg, omsg = Some msg ∧ m_sender msg ≠ saA))) as [Hempty|Hwrong]].
+    - iDestruct "Hmsg" as "[(-> & %Heq & Hsh & HRT)|(%msg' & -> & %Heq & %Heqdest & Hsh & HRT & Hnew)]".
+      { simplify_eq. naive_solver. }
+      destruct Hgood as (?&Hbody&?&?). simplify_eq.
+      iApply (mu_step_model _ _ _ _ ∅ ∅ _ ((stA, BSending (1 + (1 + n))) : stenning_model) with "Hmod [Hf] [Hfr //]").
+      { constructor. exists msg'. naive_solver. }
+      { set_solver. }
+      { set_solver. }
+      { rewrite fmap_empty map_union_empty. done. }
+      iIntros "Hmod Hf Hfr".
+      rewrite map_union_empty /usr_fl /=.
+      iMod (token_update with "[$HstB $Hst]") as "[HstB Hst]".
+      iMod ("Hclose" with "[Hfr Hmod HstA HstB]").
+      { iNext. rewrite /retinv. iFrame. iExists _, _. iFrame. }
+      iModIntro. iApply wp_value'. do 5 wp_pure _.
+      rewrite bool_decide_true; last by do 2 f_equal.
+      do 3 wp_pure _.
+      { simpl. rewrite Hbody //. }
+      do 5 wp_pure _. rewrite bool_decide_true //. do 3 wp_pure _.
+
+      wp_bind (SendTo _ _ _).
+      iApply sswp_MU_wp_fupd.
+
+      iInv Ns as "Hi" "Hclose". iModIntro.
+      iApply (wp_send _ _ false with "[Hsh] [HRT] [HsB]")=>//=>//=>//.
+      iNext. iIntros "Hsh HRT". clear stA.
+      iDestruct "Hi" as "(Hfr & %stA & %stB & Hmod & HstA & HstB)".
+      iDestruct (token_agree with "HstB Hst") as %->.
+
+      iApply (mu_step_model _ _ _ _ ∅ ∅ _ ((stA, (BReceiving (1+(1+n)))) : stenning_model) with "Hmod [Hf] [Hfr //]").
+      { simpl. replace (Send _) with (Send (mBA $ (1 + (1 + n)) - 1)). constructor. f_equal.
+        rewrite /mBA //=. do 2 f_equal. lia. }
+      { set_solver. }
+      { set_solver. }
+      { rewrite fmap_empty map_union_empty. done. }
+      iIntros "Hmod Hf Hfr".
+
+      iMod (token_update with "[$HstB $Hst]") as "[HstB Hst]".
+      iMod ("Hclose" with "[Hfr Hmod HstA HstB]").
+      { iNext. rewrite /retinv. iFrame. iExists _, _. iFrame. }
+      rewrite map_union_empty /usr_fl /=. iModIntro. iApply wp_value'. do 3 wp_pure _.
+      iApply ("IH" with "[] [Hst] [$] [$] [] [$HRT] [$]")=>//.
+      { iPureIntro; lia. }
+      { rewrite Z.add_comm //. }
+    - iApply (mu_step_model _ _ _ _ ∅ ∅ _ ((stA, BReceiving (1+n)) : stenning_model) with "Hmod [Hf] [Hfr //]").
+      { simpl. by apply B_RecvFailEmpty. }
+      { set_solver. }
+      { set_solver. }
+      { rewrite fmap_empty map_union_empty. done. }
+      iIntros "Hmod Hf Hfr".
+      rewrite map_union_empty /usr_fl /=.
+      iMod ("Hclose" with "[Hfr Hmod HstA HstB]").
+      { iNext. rewrite /retinv. iFrame. iExists _, _. iFrame. }
+      iModIntro. iApply wp_value'.
+      iDestruct "Hmsg" as "[(-> & %Heq & Hsh & HRT)|(%msg' & -> & %Heq & %Heqdest & Hsh & HRT & Hnew)]".
+      + do 3 wp_pure _. iApply ("IH" with "[] [Hst] [$] [$] [] [$HRT] [$]")=>//.
+      + do 5 wp_pure _. rewrite bool_decide_false; last naive_solver.
+        wp_pure _. iApply ("IH" with "[] [Hst] [$] [$] [] [$HRT] [$]")=>//.
+    - iDestruct "Hmsg" as "[(-> & %Heq & Hsh & HRT)|(%msg' & -> & %Heq & %Heqdest & Hsh & HRT & Hnew)]".
+      { simplify_eq. naive_solver. }
+      simplify_eq. have ?: m_sender msg' = saA by apply NNP_P; naive_solver.
+      iApply (mu_step_model _ _ _ _ ∅ ∅ _ ((stA, BSending (1 + n)) : stenning_model) with "Hmod [Hf] [Hfr //]").
+      { constructor=>//. }
+      { set_solver. }
+      { set_solver. }
+      { rewrite fmap_empty map_union_empty. done. }
+      iIntros "Hmod Hf Hfr".
+      rewrite map_union_empty /usr_fl /=.
+      iMod (token_update with "[$HstB $Hst]") as "[HstB Hst]".
+      iMod ("Hclose" with "[Hfr Hmod HstA HstB]").
+      { iNext. rewrite /retinv. iFrame. iExists _, _. iFrame. }
+      iModIntro. iApply wp_value'. do 5 wp_pure _. rewrite bool_decide_true; last by do 2 f_equal.
+      destruct (ZOfString (m_body msg')) as [?|] eqn:Heq.
+      + do 3 wp_pure _; first by rewrite /= Heq. do 5 wp_pure _. rewrite bool_decide_false; last first.
+        { intros ?; simplify_eq. apply Hbad. rewrite /good_message Z.add_comm //. naive_solver. }
+        do 2 wp_pure _. wp_bind (SendTo _ _ _).
+        iApply sswp_MU_wp_fupd. iInv Ns as "Hi" "Hclose". iModIntro.
+        iApply (wp_send _ _ false with "[Hsh] [HRT] [HsB]")=>//=>//=>//.
+        iNext. iIntros "Hsh HRT". clear stA.
+        iDestruct "Hi" as "(Hfr & %stA & %stB & Hmod & HstA & HstB)".
+        iDestruct (token_agree with "HstB Hst") as %->.
+        iApply (mu_step_model _ _ _ _ ∅ ∅ _ ((stA, (BReceiving (1+n))) : stenning_model) with "Hmod [Hf] [Hfr //]").
+        { simpl. replace (Send _) with (Send (mBA $ (1 + n) - 1)). constructor. f_equal.
+          rewrite /mBA //=. do 2 f_equal. lia. }
+        { set_solver. }
+        { set_solver. }
+        { rewrite fmap_empty map_union_empty. done. }
+        iIntros "Hmod Hf Hfr".
+        iMod (token_update with "[$HstB $Hst]") as "[HstB Hst]".
+        iMod ("Hclose" with "[Hfr Hmod HstA HstB]").
+        { iNext. rewrite /retinv. iFrame. iExists _, _. iFrame. }
+        rewrite map_union_empty /usr_fl /=. iModIntro. iApply wp_value'. do 2 wp_pure _.
+        iApply ("IH" with "[] [Hst] [$] [$] [] [$HRT] [$]")=>//.
+      + do 3 wp_pure _; first by rewrite /= Heq. do 7 wp_pure _.
+        wp_bind (SendTo _ _ _).
+        iApply sswp_MU_wp_fupd. iInv Ns as "Hi" "Hclose". iModIntro.
+        iApply (wp_send _ _ false with "[Hsh] [HRT] [HsB]")=>//=>//=>//.
+        iNext. iIntros "Hsh HRT". clear stA.
+        iDestruct "Hi" as "(Hfr & %stA & %stB & Hmod & HstA & HstB)".
+        iDestruct (token_agree with "HstB Hst") as %->.
+        iApply (mu_step_model _ _ _ _ ∅ ∅ _ ((stA, (BReceiving (1+n))) : stenning_model) with "Hmod [Hf] [Hfr //]").
+        { simpl. replace (Send _) with (Send (mBA $ (1 + n) - 1)). constructor. f_equal.
+          rewrite /mBA //=. do 2 f_equal. lia. }
+        { set_solver. }
+        { set_solver. }
+        { rewrite fmap_empty map_union_empty. done. }
+        iIntros "Hmod Hf Hfr".
+        iMod (token_update with "[$HstB $Hst]") as "[HstB Hst]".
+        iMod ("Hclose" with "[Hfr Hmod HstA HstB]").
+        { iNext. rewrite /retinv. iFrame. iExists _, _. iFrame. }
+        rewrite map_union_empty /usr_fl /=. iModIntro. iApply wp_value'. do 2 wp_pure _.
+        iApply ("IH" with "[] [Hst] [$] [$] [] [$HRT] [$]")=>//.
+  Qed.
 End with_Σ.
